migrated DFA

Evaluation/Example/instancedriver.ml
@@ -1,0 +1,76 @@
+open Instance
+open ST.R.Ty
+open L.Lex
+
+let to_string chars =
+  let buf = Buffer.create 16 in
+  List.iter (Buffer.add_char buf) chars;
+  Buffer.contents buf
+
+let to_chars s =
+  let rec exp i l =
+    if i < 0 then l else exp (i - 1) (s.[i] :: l) in
+  exp (String.length s - 1) []
+
+let read_whole_file filename =
+    let ch = open_in filename in
+    let s = really_input_string ch (in_channel_length ch) in
+    close_in ch;
+    s
+
+let token_to_string token =
+match token with
+| label, pref -> "(" ^ (to_string label) ^ ", " ^ (to_string pref) ^ ")"
+
+let rec tokens_to_string tokens =
+match tokens with
+| [] -> ""
+| t::[] -> (token_to_string t)
+| t::ts -> (token_to_string t) ^ ",\n" ^ (tokens_to_string ts)
+
+let print_results rs =
+match rs with
+| ts, rest -> (*Printf.printf "Tokens: %s\n" (tokens_to_string ts) ;*) Printf.printf "Rest: %s\n" (to_string rest)
+
+let float_to_string f = Printf.sprintf "%.5f" f
+
+let rec times_to_string' times =
+match times with
+| [] -> ""
+| t::[] -> (float_to_string t)
+| t::ts -> (float_to_string t) ^ "," ^ (times_to_string' ts)
+
+let times_to_string times = Printf.sprintf "[%s]" (times_to_string' times)
+
+let rec print_evaluation results =
+match results with
+| fname, code_len, ts, rest_len ->
+  let oc = open_out ("results/"^fname) in
+  let ts' = times_to_string ts in
+  Printf.fprintf oc "{\n\"fname\":\"%s\",\n \"input_len\":%d,\n \"times\":%s,\n \"rest_len\":%d\n}" fname code_len ts' rest_len;
+  close_out oc
+
+let time f x =
+    let t = Sys.time() in
+    let fx = f x in
+    Sys.time() -. t
+
+let rec n_copies n x =
+match n with
+| 0 -> []
+| _ -> x :: (n_copies (n-1) x)
+
+let srus = map init_srule rus
+let lex_pre = lex' srus
+let () = Printf.printf "%.5f" (time (map init_srule) rus)
+
+let evaluate fname =
+  let code = to_chars (read_whole_file ("data/"^fname)) in
+  let codes = n_copies 1 code in
+  let ts = map (time lex_pre) codes in
+  let rest = (to_string (snd (lex_pre code))) in
+  let rest_len = (String.length rest) in
+  (fname, List.length code, ts, rest_len)
+
+let xs = Array.to_list (Sys.readdir "data")
+let ps = map (fun x -> (print_evaluation (evaluate x))) xs
