Evaluation/Example/plot.py
@@ -1,0 +1,52 @@
+from os import listdir
+from statistics import mean, stdev
+import matplotlib.pyplot as plt
+from matplotlib.figure import Figure
+import numpy as np
+import json
+input_dir = "results"
+
+def fcontent(f):
+    tmp = open(f, "r")
+    content = tmp.read()
+    tmp.close()
+    return content
+
+def poly_eq(coeffs):
+    return lambda x: sum([coeffs[i]*(x**i) for i in range(0,len(coeffs))])
+
+fs = listdir(input_dir)
+print(fs)
+fs = [input_dir+"/"+f for f in fs]
+cs = [fcontent(f) for f in fs]
+js = [json.loads(c) for c in cs]
+
+for j in js:
+    if j["rest_len"] != 0:
+        print("WARNING: {} was not processed entirely".format(j["fname"]))
+
+xs = [j["input_len"] for j in js]
+ys = [mean(j["times"]) for j in js]
+# e = [stdev(j["times"]) for j in js]
+e = [0 for j in js]
+
+# for p in list(zip(xs,ys)):
+#     print("{} {}".format(p[0], p[1]))
+
+zs = np.polyfit(xs,ys,2)
+f = poly_eq(zs[::-1])
+fxs = np.arange(0,max(xs),100)
+fys = [f(x) for x in fxs]
+
+fig = plt.figure(figsize=(6,3))
+axis = fig.add_subplot(1, 1, 1)
+
+axis.plot(fxs,fys)
+axis.errorbar(xs, ys, yerr=e, fmt='ro', ms=4)
+
+axis.legend(["quadratic fit"])
+axis.set_xlabel("# Characters")
+axis.set_ylabel("Processing Time (s)")
+
+plt.tight_layout()
+plt.show()
