Verbatim/regex.v
@@ -5,17 +5,19 @@ Require Import Coq.Program.Wf.
 Require Import Coq.omega.Omega.
 
 From Verbatim Require Import ltac.
+From Verbatim Require Import order.
 
 Module Type SIGMA.
   Parameter Sigma : Type.
   Parameter SigmaEnum : list Sigma.
-  Hypothesis Sigma_finite : forall a, In a SigmaEnum.
-  Hypothesis Sigma_dec : forall(a a' : Sigma), {a = a'} + {a <> a'}.
+  Parameter Sigma_order : Sigma -> Sigma -> order.
+  Parameter Sigma_finite : forall a, In a SigmaEnum.
+  Parameter Sigma_dec : forall(a a' : Sigma), {a = a'} + {a <> a'}.
 End SIGMA.
 
 Module DefsFn (Ty : SIGMA).
 
-  Include Ty.
+  Import Ty.
 
   Module Export Strings.
 
@@ -209,6 +211,462 @@ Module DefsFn (Ty : SIGMA).
 
     End MatchSpec.
 
+    Module Export MatchSpecLemmas.
+      
+      Theorem nullable_bridge : forall(r : regex),
+        true = nullable r <-> exp_match [] r.
+      Proof.
+        intros r. split; intros H.
+        - induction r; try(simpl in H; discriminate).
+          + apply MEmpty.
+          + simpl in H. destruct (nullable r1); destruct (nullable r2); try(simpl in H; discriminate).
+            rewrite <- nil_left with (s := []). apply MApp.
+            * apply IHr1. reflexivity.
+            * apply IHr2. reflexivity.
+          + simpl in H.  destruct (nullable r1); destruct (nullable r2).
+            * apply MUnionL. apply IHr1. reflexivity.
+            * apply MUnionL. apply IHr1. reflexivity.
+            * apply MUnionR. apply IHr2. reflexivity.
+            * simpl in H. discriminate.
+          + apply MStar0.
+        - induction r.
+          + inversion H.
+          + simpl. reflexivity.
+          + inversion H.
+          + simpl. inversion H. apply empty_app in H1. destruct H1.
+            rewrite H1 in H3. rewrite H5 in H4.
+            apply IHr1 in H3. apply IHr2 in H4.
+            rewrite <- H3. rewrite <- H4. simpl. reflexivity.
+          + simpl. inversion H.
+            * apply IHr1 in H2. rewrite <- H2. destruct (nullable r2); simpl; reflexivity.
+            * apply IHr2 in H1. rewrite <- H1. destruct (nullable r1); simpl; reflexivity.
+          + simpl. reflexivity.
+      Qed.
+
+      Theorem nullable_bridge' : forall(r : regex),
+          nullable r = true <-> exp_match [] r.
+      Proof.
+        split; intros.
+        - symmetry in H. apply nullable_bridge; auto.
+        - symmetry. apply nullable_bridge; auto.
+      Qed.
+
+      
+      
+
+      (* star_concat upto concat_star necessary for hard star case of der_match *)
+      Lemma star_concat :
+        forall s r',
+          exp_match s (Star r')
+          -> (exists xss : list (list Sigma),
+                s = concat xss
+                /\ (forall xs,
+                      In xs xss
+                      -> exp_match xs r')).
+      Proof.
+        intros s r' hm.
+        remember (Star r') as r. generalize dependent r'.
+        induction hm; intros r' heq; inv heq.
+        - exists []; split; auto.
+          intros xs hi; inv hi.
+        - destruct (IHhm2 r') as (xss' & heq & hall); subst; auto.
+          exists (s1 :: xss'); split; auto.
+          intros xs hi.
+          destruct hi as [hh| ht]; subst; auto.
+      Qed.
+
+      Lemma star_concat_no_empt : forall(s : String) (r' : regex),
+          s <> []
+          -> exp_match s (Star r')
+          -> (exists xss : list (list Sigma),
+                s = concat xss
+                /\ (forall xs,
+                      In xs xss
+                      -> exp_match xs r' /\ xs <> [])).
+      Proof.
+        intros s r' Hempty Hstar. apply star_concat in Hstar.
+        destruct Hstar as (yss & heq & hall).
+        exists(rm_empty yss). split.
+        - rewrite rm_empty_mute. apply heq.
+        - intros xs H. split.
+          + apply hall.  apply filtered_subset in H. apply H.
+          + apply rm_empty_no_empty in H. apply H.
+      Qed.
+
+      Lemma concat_star : forall(xss : list String) (r : regex),
+          (forall xs : list Sigma, In xs xss -> exp_match xs r) -> exp_match (concat xss) (Star r).
+      Proof.
+        intros xss r H. induction xss.
+        - simpl. apply MStar0.
+        - replace (concat (a :: xss)) with (a ++ (concat xss)).
+          + apply MStarApp.
+            * apply H. simpl. left. reflexivity.
+            * apply IHxss. intros xs H1. apply H. simpl. right. apply H1.
+          + simpl. reflexivity.
+      Qed.
+
+      Theorem der_match : forall(a : Sigma) (s : String) (r : regex),
+          exp_match (a::s) r <-> exp_match s (derivative a r).
+      Proof.
+        intros a s r.
+        split.
+        {
+          generalize dependent s. induction r; intros s H.
+          - inv H.
+          - inv H.
+          - destruct s.
+            + simpl. destruct (Sigma_dec t a).
+              * apply MEmpty.
+              * inv H. contradiction.
+            + inv H.
+          - simpl. destruct(nullable r1) eqn:E.
+            + inv H. destruct s1.
+              * apply MUnionR. apply IHr2. rewrite <- H1. simpl. apply H4.
+              * apply MUnionL. simpl in H1. injection H1. intros Happ Hchar.
+                rewrite <- Happ. rewrite Hchar in H3. apply IHr1 in H3.
+                apply MApp.
+                -- apply H3.
+                -- apply H4.
+            + inv H. destruct s1.
+              * apply nullable_bridge in H3. rewrite E in H3. discriminate.
+              * simpl in H1. injection H1. intros Happ Hchar.
+                rewrite <- Happ. rewrite Hchar in H3. apply IHr1 in H3.
+                apply MApp.
+                -- apply H3.
+                -- apply H4.
+          - simpl. inv H.
+            + apply IHr1 in H2. apply MUnionL. apply H2.
+            + apply IHr2 in H1. apply MUnionR. apply H1.
+          (* hard_star: This case was the hard one *)
+          - apply star_concat_no_empt in H. destruct H as (xss & heq & hall).
+            + assert (H : exists(s1 : String) (yss : list String),
+                         ((a :: s1) :: yss) = xss).
+              {
+                destruct xss.
+                - simpl in heq. discriminate.
+                - simpl in heq. destruct l eqn:E.
+                  + apply hall in E.
+                    * contradiction.
+                    * rewrite E. simpl. left. reflexivity.
+                  + exists(l0). exists(xss). simpl in heq.
+                    injection heq. intros I1 I2. rewrite I2. reflexivity.
+              }
+              destruct H as [s1]. destruct H as [yss].
+              rewrite <- H in hall.
+              assert (A : In (a :: s1) ((a :: s1) :: yss)).
+              { simpl. left. reflexivity. }
+              simpl. replace s with (s1 ++ (concat yss)).
+              * apply MApp.
+                -- apply IHr. apply hall in A. destruct A. apply H0.
+                -- rewrite H in hall.
+                   assert (A1 : forall xs : list Sigma, In xs xss -> exp_match xs r).
+                   { intros xs. intros HA1. apply hall in HA1. destruct HA1. apply H0. }
+                   apply concat_star. intros xs H1. apply A1.
+                   rewrite <- H. simpl. right. apply H1.
+              * assert (A1 : concat ((a :: s1) :: yss) = concat xss).
+                { rewrite H. reflexivity. }
+                assert (A2 : concat ((a :: s1) :: yss) = a :: (s1 ++ (concat yss))).
+                { simpl. reflexivity. }
+                rewrite <- A1 in heq. rewrite A2 in heq. injection heq.
+                intros I. symmetry. apply I.
+            + unfold not. intros C. discriminate.
+        }
+        {
+          generalize dependent s. induction r; intros s H.
+          - inv H.
+          - inv H.
+          - simpl in H. destruct (Sigma_dec t a); inv H. apply MChar.
+          - simpl in H. destruct (nullable r1) eqn:E.
+            + inv H.
+              * inv H2. replace (a :: s1 ++ s2) with ((a :: s1) ++ s2).
+                apply MApp.
+                -- apply IHr1. apply H3.
+                -- apply H4.
+                -- reflexivity.
+              * symmetry in E. apply nullable_bridge in E. rewrite <- nil_left with (s := (a :: s)).
+                apply MApp.
+                -- apply E.
+                -- apply IHr2. apply H1.
+            + inv H.
+              * replace (a :: s1 ++ s2) with ((a :: s1) ++ s2).
+                apply MApp.
+                -- apply IHr1. apply H3.
+                -- apply H4.
+                -- reflexivity.
+          - inv H.
+            + apply MUnionL. apply IHr1. apply H2.
+            + apply MUnionR. apply IHr2. apply H1.
+          - simpl in H. inv H. replace (a :: s1 ++ s2) with ((a :: s1) ++ s2).
+            + apply MStarApp.
+              * apply IHr. apply H3.
+              * apply H4.
+            + reflexivity.
+        }
+      Qed.
+      
+    End MatchSpecLemmas.
+
+    Module Notations.
+      
+      Notation "e1 = e2 " := (regex_eq e1 e2) (at level 70).
+      Notation "a ∂ r" := (derivative a r) (at level 75, right associativity).
+      Notation ε := EmptyStr.
+      Notation "e1 @ e2" := (App e1 e2) (at level 75).
+      Notation "e1 # e2" := (Union e1 e2) (at level 75).
+
+    End Notations.
+
+    Module Helpers.
+      
+      Definition Plus (r : regex) : regex := App r (Star r).
+
+      Fixpoint IterUnion (rs : list regex) :=
+        match rs with
+        | [] => EmptySet
+        | [e] => e
+        | h::t => Union h (IterUnion t)
+        end.
+
+      Fixpoint IterApp (rs : list regex) :=
+        match rs with
+        | [] => EmptyStr
+        | [e] => e
+        | h::t => App h (IterApp t)
+        end.
+
+      (* r? *)
+      Definition Optional (r : regex) := Union EmptyStr r.
+
+      Definition REString (z : String) := IterApp (map Char z).
+
+    End Helpers.
+
+    Module Export Similarity.
+
+      Module Export Spec.
+
+        Inductive re_sim_prop : regex -> regex ->  Prop
+          :=
+            u_self1 (r : regex) : re_sim_prop (Union r r) r
+          | u_self2 (r : regex) : re_sim_prop r (Union r r)
+          | u_comm1 (r s : regex) : re_sim_prop (Union r s) (Union s r)
+          | u_comm2 (r s : regex) : re_sim_prop (Union s r) (Union r s)
+          | u_assoc1 (r s t : regex) :
+              re_sim_prop (Union (Union r s) t) (Union r (Union s t))
+          | u_assoc2 (r s t : regex) :
+              re_sim_prop (Union r (Union s t)) (Union (Union r s) t)
+          | a_assoc1 (r s t : regex) :
+              re_sim_prop (App (App r s) t) (App r (App s t))
+          | a_assoc2 (r s t : regex) :
+              re_sim_prop (App r (App s t)) (App (App r s) t)
+          | sim_refl (r : regex) : re_sim_prop r r.
+
+      End Spec.
+
+      Module Export Impl.
+
+        Import Notations.
+
+        Definition re_sim (e1 e2 : regex) : bool :=
+          (e1 = e2)                                       (* sim refl *)
+          || match e1, e2 with
+            | (r1 # s1) # (t1 # u1), (r2 # s2) # (t2 # u2) =>
+              (  (e1 = (r2 # s2)) && (e1 = (t2 # u2))  ) (* self union *)
+              || (  (e2 = (r1 # s1)) && (e2 = (t1 # u1))  ) (* self union *)
+              || (  ((r1 # s1) = (t2 # u2)) && ((t1 # u1) = (r2 # s2))  ) (* union commutes *)
+              (** treat (r1 # s1) as r1 and (t2 # u2) as t2, as in case 2 **)
+              || (  ((r1 # s1) = r2) && (t1 = s2) && (u1 = (t2 # u2))  ) (* union assoc *)
+              (** treat (r2 # s2) as r2 and (t1 # u1) as t1, as in case 3 **)
+              || (  (r1 = (r2 # s2)) && (s1 = t2) && ((t1 # u1) = u2)  ) (* union assoc *)
+            (* * case 2 * *)
+            | r1 # (s1 # t1), (r2 # s2) # t2 =>
+              (  (e1 = (r2 # s2)) && (e1 = t2)  )          (* self union *)
+              || (  (e2 = r1) && (e2 = (s1 # t1))  )        (* self union *)
+              || (  (r1 = t2) && ((s1 # t1) = (r2 # s2))  ) (* union commutes *)
+              || (  (r1 = r2) && (s1 = s2) && (t1 = t2)  )  (* union assoc *)
+            (* * case 3 * *)
+            | (r1 # s1) # t1, r2 # (s2 # t2) =>
+              (  (e1 = r2) && (e1 = (s2 # t2))  )          (* self union *)
+              || (  (e2 = (r1 # s1)) && (e2 = t1)  )        (* self union *)
+              || (  ((r1 # s1) = (s2 # t2)) && (t1 = r2)  ) (* union commutes *)
+              || (  (r1 = r2) && (s1 = s2) && (t1 = t2)  )  (* union assoc *)
+            | r1 # s1, s2 # r2 =>
+              (  (e1 = r2) && (e1 = s2)  )                 (* self union *)
+              || (  (e2 = r1) && (e2 = s1)  )                (* self union *)
+              || (  (r1 = r2) && (s1 = s2)  )                (* union commutes *)
+            | r0 # r1, _ =>
+              (  (e2 = r0) && (e2 = r1)  )                  (* self union *)
+            | _, r0 # r1 =>
+              (  (e1 = r0) && (e1 = r1)  )                  (* self union *)
+            | (r1 @ s1) @ (t1 @ u1), (r2 @ s2) @ (t2 @ u2) =>
+              (  ((r1 @ s1) = r2) && (t1 = s2) && (u1 = (t2 @ u2))  )
+              || (  (r1 = (r2 @ s2)) && (s1 = t2) && ((t1 @ u1) = u2)  )
+            | r1 @ (s1 @ t1), (r2 @ s2) @ t2 =>
+              (  (r1 = r2) && (s1 = s2) && (t1 = t2)  )     (* assoc commutes *)                           
+            | (r1 @ s1) @ t1, r2 @ (s2 @ t2) => 
+              (  (r1 = r2) && (s1 = s2) && (t1 = t2)  )     (* assoc commutes *)   
+            | _, _ => false
+            end.
+
+      End Impl.
+
+      Module Lemmas.
+
+        Theorem re_sim_correctF : forall e1 e2,
+          re_sim e1 e2 = true -> re_sim_prop e1 e2.
+        Proof.
+          intros.
+          unfold re_sim in H.
+          repeat dm; try(discriminate);
+            repeat(first [rewrite Bool.orb_true_iff in *; destruct H
+                         | rewrite Bool.andb_true_iff in *; destruct H]);
+            try(discriminate);
+            try(rewrite <- regex_eq_correct in *; discriminate);
+            try(rewrite <- regex_eq_correct in *; subst; constructor);
+            try(rewrite <- regex_eq_correct in *; rewrite H; constructor);
+            try(rewrite <- regex_eq_correct in *; rewrite H0; constructor);
+            try(rewrite <- regex_eq_correct in *; rewrite H; rewrite H0; constructor);
+            try(rewrite <- regex_eq_correct in *; rewrite <- H; rewrite <- H0; constructor).
+        Qed.
+  
+        Theorem re_sim_correctB : forall e1 e2,
+            re_sim_prop e1 e2 -> re_sim e1 e2 = true.
+        Proof.
+          intros.
+          inv H; try(eapply re_sim_correctB_trans; eauto; reflexivity);
+            unfold re_sim;
+            try(rewrite Bool.orb_true_iff; left; rewrite <- regex_eq_correct; reflexivity);
+            repeat dm; try(discriminate);
+              repeat(first [rewrite Bool.orb_true_iff | rewrite Bool.andb_true_iff]);
+              repeat(rewrite <- regex_eq_correct); repeat rewrite regex_eq_refl;
+                try(right; right; right; right; right; split; reflexivity);
+                try(right; left; right; right; right; split; reflexivity);
+                try(left; right; right; right; right; split; reflexivity);
+                try(left; left; right; right; right; split; reflexivity);
+                try(right; right; right; right; left; split; reflexivity);
+                try(right; left; right; right; left; split; reflexivity);
+                try(left; right; right; right; left; split; reflexivity);
+                try(left; left; right; right; left; split; reflexivity);
+                try(right; right; right; left; right; split; reflexivity);
+                try(right; left; right; left; right; split; reflexivity);
+                try(left; right; right; left; right; split; reflexivity);
+                try(left; left; right; left; right; split; reflexivity);
+                try(right; right; right; left; left; split; reflexivity);
+                try(right; left; right; left; left; split; reflexivity);
+                try(left; right; right; left; left; split; reflexivity);
+                try(left; left; right; left; left; split; reflexivity);
+                try(right; right; left; right; right; split; reflexivity);
+                try(right; left; left; right; right; split; reflexivity);
+                try(left; right; left; right; right; split; reflexivity);
+                try(left; left; left; right; right; split; reflexivity);
+                try(right; right; left; right; left; split; reflexivity);
+                try(right; left; left; right; left; split; reflexivity);
+                try(left; right; left; right; left; split; reflexivity);
+                try(left; left; left; right; left; split; reflexivity);
+                try(right; right; left; left; right; split; reflexivity);
+                try(right; left; left; left; right; split; reflexivity);
+                try(left; right; left; left; right; split; reflexivity);
+                try(left; left; left; left; right; split; reflexivity);
+                try(right; right; left; left; left; split; reflexivity);
+                try(right; left; left; left; left; split; reflexivity);
+                try(left; right; left; left; left; split; reflexivity);
+                try(left; left; left; left; left; split; reflexivity);
+                try(right; left; left; left; right; split; reflexivity);
+                try(right; right; right; right; split; reflexivity);
+                try(right; right; right; left; split; reflexivity);
+                try(right; right; left; right; split; reflexivity);
+                try(right; right; left; left; split; reflexivity);
+                try(right; left; right; right; split; reflexivity);
+                try(right; left; right; left; split; reflexivity);
+                try(right; left; left; right; split; reflexivity);
+                try(right; left; left; left; split; reflexivity);
+                try(left; right; right; right; split; reflexivity);
+                try(left; right; right; left; split; reflexivity);
+                try(left; right; left; right; split; reflexivity);
+                try(left; right; left; left; split; reflexivity);
+                try(left; left; right; right; split; reflexivity);
+                try(left; left; right; left; split; reflexivity);
+                try(left; left; left; right; split; reflexivity);
+                try(left; left; left; left; split; reflexivity);
+                try(right; right; right; split; reflexivity);
+                try(right; right; left; split; reflexivity);
+                try(right; left; right; split; auto; reflexivity);
+                try(right; left; left; split; reflexivity);
+                try(left; right; right; split; reflexivity);
+                try(left; right; left; split; reflexivity);
+                try(left; left; right; split; reflexivity);
+                try(left; left; left; split; reflexivity);
+                try(right; right; split; reflexivity);
+                try(right; right; split; auto; reflexivity);
+                try(right; left; split; auto; reflexivity);
+                try(left; right; split; reflexivity);
+                try(left; left; split; reflexivity);
+                try(left; split; reflexivity);
+                try(right; split; auto; reflexivity).
+        Qed.
+
+      End Lemmas.
+
+      Module Export Correct.
+
+        Import Lemmas.
+
+        Theorem re_sim_correct : forall e1 e2,
+            re_sim e1 e2 = true <-> re_sim_prop e1 e2.
+        Proof.
+          intros; split; [apply re_sim_correctF | apply re_sim_correctB].
+        Qed.
+
+        Lemma re_sim_refl : forall e, re_sim e e = true.
+        Proof.
+          intros. rewrite re_sim_correct. constructor.
+        Qed.
+
+        Theorem re_sim_symm : forall e1 e2, re_sim e1 e2 = re_sim e2 e1.
+        Proof.
+          intros. destruct (re_sim e1 e2) eqn:E; symmetry.
+          - rewrite re_sim_correct in *. inv E; constructor.
+          - rewrite false_not_true in *. intros C. destruct E.
+            rewrite re_sim_correct in *. inv C; constructor.
+        Qed.
+        
+        Theorem re_sim_equiv : forall e1 e2,
+            re_sim e1 e2 = true -> re_equiv e1 e2.
+        Proof.
+          intros. apply re_sim_correct in H.
+          inv H;
+            try(unfold re_equiv; intros; split; intros;
+                inv H; auto; repeat(constructor); auto; reflexivity);
+            unfold re_equiv; intros; split; intros.
+          - inv H.
+            + inv H2.
+              * apply MUnionL. auto.
+              * apply MUnionR. apply MUnionL. auto.
+            + apply MUnionR. apply MUnionR. auto.
+          - inv H.
+            + apply MUnionL. apply MUnionL. auto.
+            + inv H1.
+              * apply MUnionL. apply MUnionR. auto.
+              * apply MUnionR. auto.
+          - inv H.
+            + apply MUnionL. apply MUnionL. auto.
+            + inv H1.
+              * apply MUnionL. apply MUnionR. auto.
+              * apply MUnionR. auto.
+          - inv H.
+            + inv H2.
+              * apply MUnionL. auto.
+              * apply MUnionR. apply MUnionL. auto.
+            + apply MUnionR. apply MUnionR. auto.
+          - inv H. inv H3. rewrite <- app_assoc. repeat(constructor); auto.
+          - inv H. inv H4. rewrite app_assoc. repeat(constructor); auto.
+          - inv H. inv H4. rewrite app_assoc. repeat(constructor); auto.
+          - inv H. inv H3. rewrite <- app_assoc. repeat(constructor); auto.
+        Qed.
+
+      End Correct.
+
+    End Similarity.
 
 End DefsFn.
 
@@ -220,6 +678,5 @@ End DefsT.
 Module Type T.
   Declare Module Ty : SIGMA.
   Declare Module Defs  : DefsT Ty.
-  Export Ty.
   Export Defs.
 End T.
