Utils/asciiFinite.v
@@ -1,0 +1,20 @@
+Require Import List.
+Import ListNotations.
+Require Import Ascii.
+
+
+Fixpoint asciiEnumFn (n : nat) : list ascii :=
+        match n with
+        | 0 => []
+        | S m => (ascii_of_nat m) :: asciiEnumFn m
+        end.
+
+Definition asciiEnum : list ascii := asciiEnumFn 256.
+
+Lemma ascii_finite : forall a : ascii, In a asciiEnum.
+Proof.
+  intros. destruct a.
+  destruct b; destruct b0; destruct b1; destruct b2;
+    destruct b3; destruct b4; destruct b5; destruct b6;
+      repeat(try(left; reflexivity); right).
+Qed.
