Utils/ascii_order.v
@@ -1,0 +1,34 @@
+Require Import List.
+Import ListNotations.
+Require Import Ascii.
+
+From Verbatim Require Import Utils.order.
+
+Definition ascii2list (a : ascii) : list bool :=
+  match a with
+  | Ascii b b0 b1 b2 b3 b4 b5 b6 =>
+    [b; b0; b1; b2; b3; b4; b5; b6]
+  end.
+
+Definition bool_order (b1 b2 : bool) : order :=
+  match b1, b2 with
+  | false, false => EQUAL
+  | false, true => LESSER
+  | true, false => GREATER
+  | true, true => EQUAL
+  end.
+  
+Fixpoint bool_list_order (bs bs' : list bool) : order :=
+  match bs, bs' with
+  | [], [] => EQUAL
+  | [], _ => LESSER
+  | _, [] => GREATER
+  | h :: t, h' :: t' =>
+    match bool_order h h' with
+    | EQUAL => bool_list_order t t'
+    | o => o
+    end
+  end.
+
+Definition ascii_order (a1 a2 : ascii) : order :=
+  bool_list_order (ascii2list a1) (ascii2list a2).
