Utils/order.v
@@ -1,0 +1,4 @@
+Inductive order :=
+    | LESSER
+    | EQUAL
+    | GREATER.
