Verbatim/DFA/DFA.v
@@ -1,0 +1,255 @@
+Require Import List.
+Import ListNotations.
+Require Import PeanoNat.
+Require Import Coq.omega.Omega.
+
+From Verbatim Require Import ltac.
+From Verbatim Require Import regex.
+From Verbatim Require Import matcher.
+From Verbatim Require Import Table.
+
+Module DFAFn (TabT : Table.T).
+
+  Import TabT.
+  Import TabT.Defs.
+
+  Module Export CoreDefs.
+
+    Fixpoint char_set (e : regex) : list Sigma :=
+      match e with
+      | EmptySet | EmptyStr => []
+      | Char a => [a]
+      | Union e1 e2 | App e1 e2 => nodup Sigma_dec ((char_set e1) ++ (char_set e2))
+      | Star e1 => char_set e1
+      end.
+
+    Fixpoint regex_depth (e : regex) : nat := 
+      match e with
+      | EmptySet
+      | EmptyStr
+      | Char _ => 0
+      | App e1 e2
+      | Union e1 e2 =>
+        let
+          d1 := regex_depth e1 in
+        let
+          d2 := regex_depth e2 in
+        if leb d2 d1 then d1 + 1 else d2 + 1
+      | Star e0 => (regex_depth e0) + 1
+      end.
+    
+    Fixpoint fin_states (es : list regex) :=
+      match es with
+      | [] => []
+      | h :: t =>
+        let t' := fin_states t in
+        if nullable h
+        then h :: t'
+        else t'
+      end.
+
+    Definition DFA : Type := regex * Table * list regex.
+    Definition defDFA : DFA := (EmptySet, emptyTable, []).
+
+    Definition DFAtransition (a : Sigma) (dfa : DFA) : DFA :=
+      match dfa with
+        (e, T, fins)
+        => match get_Table T e a with
+          | Some e' => (e', T, fins)
+          | None => (derivative a e, T, fins)
+          end
+      end.
+
+    Fixpoint DFAtransition_list (bs : list Sigma) (dfa : DFA) : DFA :=
+      match bs with
+      | [] => dfa
+      | c :: cs => DFAtransition_list cs (DFAtransition c dfa)
+      end.
+
+    Definition DFAaccepting (dfa : DFA) : bool :=
+      match dfa with
+        (e, T, fins)
+        => match find (fun x => regex_eq e x) fins with
+          | None => nullable e
+          | Some _ => true
+          end
+      end.
+
+    Fixpoint DFAaccepts (z : String) (dfa : DFA) : bool :=
+      match z with
+      | [] => DFAaccepting dfa
+      | x :: xs => DFAaccepts xs (DFAtransition x dfa)
+      end.
+
+    Definition regex2dfa (e : regex) : DFA :=
+      let
+        T := fill_Table_all emptyTable e (char_set e) ((regex_depth e)^2)
+      in
+      let
+        es := get_states T
+      in
+      (canon e, T, fin_states es).
+    
+    Definition dfa2regex (dfa : DFA) : regex :=
+      match dfa with (e, _, _) => e end.
+
+  End CoreDefs.
+
+  Module Export Correct.
+
+    Module Import Mat := MatcherFn TabT.R.
+
+    Lemma re_sim_nullable : forall e e',
+      re_sim e e' = true
+      -> nullable e = nullable e'.
+    Proof.
+      intros. apply re_sim_equiv in H.
+      unfold re_equiv in H. specialize (H []).
+      do 2 rewrite <- nullable_bridge in H.
+      apply Bool.eq_true_iff_eq. split; intros; symmetry; apply H; symmetry; auto.
+    Qed.
+
+    Lemma In_fin_nullable : forall es x,
+      In x (fin_states es)
+      -> nullable x = true.
+    Proof.
+      induction es; intros.
+      - contradiction.
+      - simpl in H. destruct (nullable a) eqn:E.
+        + simpl in H. destruct H.
+          * subst; auto.
+          * auto.
+        + auto.
+    Qed.
+
+    Theorem DFAaccepting_nullable : forall es T e,
+      DFAaccepting (e, T, fin_states es) = nullable e.
+    Proof.
+      intros. unfold DFAaccepting. dm.
+      apply find_some in E. destruct E.
+      apply In_fin_nullable in H.
+      apply regex_eq_correct in H0.
+      symmetry in H. rewrite H0 in *; auto.
+    Qed.
+
+    Theorem transition_Table_correct : forall e e' T es,
+        regex2dfa e = (e', T, es)
+        -> derived T /\ (exists es', es = fin_states es') /\ canon e = e'.
+    Proof.
+      intros. 
+      unfold regex2dfa in *. injection H; intros.
+      repeat(split).
+      - apply derived_get_some in H3.
+        + apply H3.
+        + eapply derived_closure_all; eauto. apply emptyTable_derived.
+      - apply derived_get_some in H3.
+        + apply H3.
+        + eapply derived_closure_all; eauto. apply emptyTable_derived.
+      - eexists; eauto.
+      - auto.
+    Qed.
+
+    Theorem transition_deriv : forall es es' e e' T T' a,
+        derived T
+        -> DFAtransition a (e, T, es) = (e', T', es')
+        -> re_equiv (derivative a e) e'
+          /\ T = T' /\ es = es'.
+    Proof.
+      intros. unfold derived in *. unfold DFAtransition in *. dm.
+      - injection H0; intros; subst. clear H0.
+        apply H in E. split; [|split]; auto.
+        unfold re_equiv in *. intros. symmetry. auto.
+      - injection H0; intros; subst. inv H0.
+        split; [| split]; auto. unfold re_equiv. reflexivity.
+    Qed.
+
+    Lemma accepts_cons : forall z a dfa,
+        DFAaccepts (a :: z) dfa
+        = DFAaccepts z (DFAtransition a dfa).
+    Proof.
+      auto.
+    Qed.
+
+    Lemma unfold_transition_list : forall bs a dfa,
+        DFAtransition_list bs (DFAtransition a dfa)
+        = DFAtransition_list (a :: bs) dfa.
+    Proof.
+      auto.
+    Qed.
+    
+    Lemma accepts_str_lst : forall z dfa,
+        DFAaccepts z dfa = DFAaccepting (DFAtransition_list z dfa).
+    Proof.
+      induction z; intros; auto.
+      rewrite accepts_cons. rewrite <- unfold_transition_list.
+      apply IHz.
+    Qed.
+    
+    Theorem accepts_deriv : forall z es T e a,
+        (forall (es : list regex) (T : Table) (e : regex),
+            derived T -> DFAaccepts z (e, T, fin_states es) = exp_matchb z e)
+        -> derived T
+        -> DFAaccepts (a :: z) (e, T, fin_states es)
+          = DFAaccepts z (derivative a e, T, fin_states es).
+    Proof.
+      intros. rewrite accepts_cons. do 2 rewrite accepts_str_lst.
+      unfold DFAtransition. repeat dm.
+      do 2 rewrite <- accepts_str_lst.
+      rewrite H; auto. rewrite H; auto.
+      apply derived_get_some in E; auto.
+      unfold re_equiv in E.
+      destruct (exp_matchb z r) eqn:E1.
+      - symmetry in E1. rewrite match_iff_matchb in *. apply E. auto.
+      - symmetry. rewrite false_not_true in *. intros C. destruct E1.
+        symmetry. symmetry in C. rewrite match_iff_matchb in *. apply E. auto.
+    Qed.
+
+    Theorem accepts_matchb : forall z es T e,
+        derived T
+        -> DFAaccepts z (e, T, fin_states es)
+          = exp_matchb z e.
+    Proof.
+      induction z; intros.
+      - simpl. dm. apply find_some in E; destruct E.
+        apply In_fin_nullable in H0.
+        apply regex_eq_correct in H1. rewrite H1. auto.
+      - rewrite accepts_deriv; auto.
+        rewrite der_matchb'; auto.
+    Qed.
+
+    Theorem accepts_match : forall z es T e,
+        derived T ->
+        (DFAaccepts z (e, T, fin_states es) = true <-> exp_match z e).
+    Proof.
+      intros. rewrite accepts_matchb; auto.
+      rewrite <- match_iff_matchb. split; symmetry; auto.
+    Qed.
+
+    Theorem r2d_accepts_match : forall z e,
+        DFAaccepts z (regex2dfa e) = true <-> exp_match z e.
+    Proof.
+      intros. destruct regex2dfa eqn:H0. destruct p. apply transition_Table_correct in H0.
+      do 3 destruct H0. subst.
+      rewrite accepts_match; auto.
+      apply canon_equiv.
+    Qed.
+
+    (*  exp_match s (dfa2regex (regex2dfa r)) <-> exp_match s r *)
+
+    (* true = accepts s fsm <-> exp_match s (dfa2regex fsm) *)
+    (*
+    Lemma foo : forall z dfa,
+        DFAaccepts z dfa = DFAaccepts z (regex2dfa (dfa2regex dfa)).
+    Proof.
+      intros. destruct dfa. destruct p. simpl.
+    Qed.*)
+
+    (*
+    Theorem d2r_accepts_match : forall z dfa,
+        DFAaccepts z dfa = true <-> exp_match z (dfa2regex dfa).
+    Proof.
+      intros.*)
+
+  End Correct.
+
+End DFAFn.
