Verbatim/DFA/Table.v
@@ -1,0 +1,524 @@
+Require Import List.
+Import ListNotations.
+Require Import Coq.Program.Wf.
+Require Import Coq.omega.Omega.
+
+
+From Verbatim Require Import ltac.
+From Verbatim Require Import Utils.order.
+From Verbatim Require Import regex.
+
+Module Type TABLE (R : regex.T).
+
+  Import R.Ty.
+  Import R.Defs.
+
+  Parameter Table : Type.
+  Parameter emptyTable : Table.
+  (*The first regex is for indexing, the second is the content of the cell*)
+  Parameter set_Table : Table -> regex -> Sigma -> regex -> Table.
+  Parameter get_Table : Table -> regex -> Sigma -> option (regex).
+
+  Parameter correct_Table : forall T e a r, get_Table (set_Table T e a r) e a = Some (r).
+  Parameter moot_setTable : forall T e0 e a b r,
+      a <> b
+      \/ e <> e0
+      -> get_Table (set_Table T e b r) e0 a = get_Table T e0 a.
+  Parameter correct_emptyTable : forall e a, get_Table emptyTable e a = None.
+
+
+  Parameter add_state : Table -> regex -> Table.
+  Parameter get_states : Table -> list regex.
+  Parameter empty_states : get_states emptyTable = [].
+  Parameter correct_states : forall T r, In r (get_states (add_state T r)).
+  Parameter moot_add_state : forall T e a r,
+      get_Table T e a = get_Table (add_state T r) e a.
+  (* might need a hypothesis about not being in states *)
+
+End TABLE.
+
+Module DefsFn (R : regex.T) (TabTy : TABLE R).
+
+  Import TabTy.
+  Import R.Defs.
+  Import R.Ty.
+
+  Module Export Get_Sim.
+    (*
+    Fixpoint get_sim' (es : list regex) (e : regex) : option regex :=
+      match es with
+      | [] => None
+      | h :: t => if re_sim e h then Some h else get_sim' t e
+      end.
+
+    Theorem get_sim'_correct : forall es e e',
+        get_sim' es e = Some e' -> In e' es /\ re_sim e e' = true.
+    Proof.
+      induction es; intros; try(discriminate).
+      simpl in H. dm.
+      - injection H; intros. rewrite H0 in *. split; simpl; auto.
+      - apply IHes in H. destruct H. split; simpl; auto.
+    Qed.
+    
+    Definition get_sim (T : Table) (e : regex) : option regex :=
+      get_sim' (get_states T) e.
+    
+    Theorem get_sim_correct : forall T e e',
+        get_sim T e = Some e' -> In e' (get_states T) /\ re_sim e e' = true.
+    Proof.
+      intros. unfold get_sim in *. apply get_sim'_correct; auto.
+    Qed.*)
+
+    (* If the regexes are ordered this can be faster *)
+    Fixpoint get_eq' (es : list regex) (e : regex) : option regex :=
+      match es with
+      | [] => None
+      | h :: t => if regex_eq e h then Some h else get_eq' t e
+      end.
+
+    Definition get_eq (T : Table) (e : regex) : option regex :=
+      get_eq' (get_states T) e.
+
+    Lemma get_eq_correct : forall T e e',
+        get_eq T e = Some e' -> In e' (get_states T) /\ regex_eq e e' = true.
+    Admitted.
+
+  End Get_Sim.
+
+  Module Export FillTable.
+
+    Import R.Defs.Helpers.
+
+    Fixpoint re_order (e1 e2 : regex) : order :=
+      match e1, e2 with
+      | EmptyStr, EmptyStr => EQUAL
+      | EmptyStr, _ => LESSER
+      | _, EmptyStr => GREATER
+      | EmptySet, EmptySet => EQUAL
+      | EmptySet, _ => LESSER
+      | _, EmptySet => GREATER
+      | Char a, Char b => Sigma_order a b
+      | Char _, _ => LESSER
+      | _, Char _ => GREATER
+      | App e1 e2, App e3 e4 =>
+        match re_order e1 e3 with
+        | EQUAL => re_order e2 e4
+        | comp => comp
+        end
+      | App _ _, _ => LESSER
+      | _, App _ _ => GREATER
+      | Star e1, Star e2 => re_order e1 e2
+      | Star _, _ => LESSER
+      | _, Star _ => GREATER
+      | Union e1 e2, Union e3 e4 =>
+        match re_order e1 e3 with
+        | EQUAL => re_order e2 e4
+        | comp => comp
+        end
+      end.
+
+    (* Assume all union inputs are already canonical:
+       1. All iterared unions are recursively right associated
+       2. All iterated unions are in lexicographic order
+       3. The EmptySet is not present in any union
+       4. All regexes in all iterated unions are unique
+     *)
+    Fixpoint mkIterUnion' (e : regex) : list regex :=
+      match e with
+      | Union e1 e2 =>
+        e1 :: (mkIterUnion' e2)
+      | _ => [e]
+      end.
+
+    Program Fixpoint merge (es1 es2 : list regex)
+            { measure ((length es1) + (length es2)) } : list regex :=
+      match es1, es2 with
+      | [], _ => es2
+      | _, [] => es1
+      | h1 :: t1, h2 :: t2 =>
+        match re_order h1 h2 with
+        | EQUAL => merge (h1 :: t1) t2
+        | LESSER => h1 :: (merge t1 (es2))
+        | GREATER => h2 :: (merge es1 t2)
+        end
+      end.
+    Next Obligation.
+      simpl. omega.
+    Defined.
+    Next Obligation.
+      simpl. omega.
+    Defined.
+      
+
+    (* Assume all App inputs and subterms are recursively right associated *)
+    Fixpoint mkIterApp' (e : regex) : list regex :=
+      match e with
+      | App e1 e2 => e1 :: (mkIterApp' e2)
+      | _ => [e]
+      end.      
+
+    (* Instead of checking for similarity, 
+       force all regexes to be in the right hand form of the relation.
+       Also use associativity/commutativity to force lexical ordering on Unioned exps
+       Then check for equality.
+     *)
+    Fixpoint canon (e : regex) : regex :=
+      match e with
+      | Union e1 e2 =>
+        match canon e1, canon e2 with
+        (* The next two patters ensure that unions don't contain EmptySet *)
+        | EmptySet, ec2 => ec2
+        | ec1, EmptySet => ec1
+        | ec1, ec2 =>
+          (* sort and make right recursive *)
+          (* Note : merge also removes duplicates *)
+          IterUnion (merge (mkIterUnion' ec1) (mkIterUnion' ec2))
+        end
+      | App e1 e2 =>
+        match canon e1, canon e2 with
+        (* The next two patterns ensure that all iterated apps
+           containing an EmptySet reduce to the EmptySet *)
+        | EmptySet, _ => EmptySet
+        | _, EmptySet => EmptySet
+        (* The next two patters ensure that apps don't contain EmptyStr *)
+        | EmptyStr, ec2 => ec2
+        | ec1, EmptyStr => ec1
+        | ec1, ec2 =>
+          IterApp ( (mkIterApp' ec1) ++ (mkIterApp' ec2) )
+        end
+      | Star EmptySet => EmptyStr
+      | Star EmptyStr => EmptyStr
+      | Star (Star r) => canon r
+      | _ => e
+      end.
+
+    Lemma canon_equiv : forall e,
+        re_equiv (canon e) e.
+    Proof.
+    Admitted.
+    
+    Fixpoint fill_Table_all' (T : Table) (e : regex) (bs : list Sigma) (fuel : nat) : Table :=
+      match fuel with
+      | 0 => T
+      | S n =>
+        let
+          (* We need a helper function to apply fill_Table_all to each derivative of e *)
+          fix fill_Table_ds (bs' : list Sigma) :=
+          match bs' with
+          | [] => T
+          | c :: cs =>
+            let
+              (* fill the table with respect to the tail *)
+              T1 := fill_Table_ds cs in
+            let
+              (* now we'll do it with respect to c *)
+              d := canon (derivative c e) in
+            (** 
+                get_sim is probably very expensive.
+                The list of states doesn't have any logical order to it right now.
+                Given a regex, there is only a small class of regexes that could be similar.
+                Should somehow bucket the list of states by these classes.
+             **)
+            (**
+               One of the paper talks about canonicalizing regexes with smart constructors.
+               I'm not sure if this is necessary for the DFA construction.
+               I can imagine how it would make similarity checks faster/bucketing easier.
+             **)
+            (**
+               Right now states are regexes. It would be better if they were integers.
+               Would need to keep track of the association between integers and regexes.
+               Maybe that should be handled by the table?
+            **)
+            match get_eq T d with
+            | None =>
+              let
+                (* we didn't find a similar regex, we need to add d *)
+                T2 := add_state T1 d in
+              let
+                (* we also need to transition from regex e to regex d on symbol c *)
+                T3 := set_Table T2 e c d in
+              (* finally we need to fill up the table with respect to d *)
+              fill_Table_all' T3 d bs n
+            | Some e' =>
+              (* In this case, we found a regex that has already been added to the table *)
+              (* Anytime we add a regex, we immediately call fill_Table_all for it *)
+              (* Therefore, we don't need to call fill_Table_all again *)
+              (* Instead, we transition from e to e' when we see c *)
+              set_Table T1 e c e'
+            end
+          end
+        in
+        fill_Table_ds bs
+      end.
+
+    Definition fill_Table_all (T : Table) (e : regex) (bs : list Sigma) (fuel : nat) : Table :=
+      fill_Table_all' T (canon e) bs fuel.
+    
+
+  End FillTable.
+
+  Module Export Spec.
+
+    Definition derived (T : Table) : Prop :=
+      forall e a r, get_Table T e a = Some r -> re_equiv r (derivative a e).
+
+  End Spec.
+
+  Module Export Correct.
+
+    Theorem emptyTable_derived : derived emptyTable.
+    Proof.
+      unfold derived. intros. rewrite correct_emptyTable in H. discriminate.
+    Qed.
+
+    Lemma unfold_filler' : forall bs T e n,
+        fill_Table_all' T e bs (S n)
+        =
+        let
+          fix fill_Table_ds (bs' : list Sigma) : Table :=
+          match bs' with
+          | [] => T
+          | c :: cs =>
+            let T1 := fill_Table_ds cs in
+            let d := canon (derivative c e) in
+            match get_eq T d with
+            | Some e' => set_Table T1 e c e'
+            | None =>
+              let T2 := add_state T1 d in
+              let T3 := set_Table T2 e c d in fill_Table_all' T3 d bs n
+            end
+          end in
+        fill_Table_ds bs.
+    Proof.
+      auto.
+    Qed.
+
+    Lemma unfold_filler_ds : forall T T' e x xs n,
+        let
+          fix fill_Table_ds (bs' : list Sigma) : Table :=
+          match bs' with
+          | [] => T
+          | c :: cs =>
+            let T1 := fill_Table_ds cs in
+            let d := canon (derivative c e) in
+            match get_eq T d with
+            | Some e' => set_Table T1 e c e'
+            | None =>
+              let T2 := add_state T1 d in
+              let T3 := set_Table T2 e c d in fill_Table_all' T3 d (x :: xs) n
+            end
+          end in
+        T' = fill_Table_ds (x :: xs)
+        ->
+        (exists e' T0, get_eq T (canon (derivative x e)) = Some e'
+                  /\ T0 = (fill_Table_ds xs)
+                  /\ T' = set_Table T0 e x e')
+        \/
+        (exists T0, get_eq T (canon (derivative x e)) = None
+               /\
+               T0 = (fill_Table_ds xs)
+               /\
+               T' = fill_Table_all'
+                      (set_Table (add_state T0 (canon (derivative x e))) e x
+                                 (canon (derivative x e)))
+                      (canon (derivative x e)) (x :: xs) n).
+    Proof.
+      intros. simpl in *. destruct (get_eq T (canon (derivative x e))) eqn:E.
+      - left. eexists; eauto.
+      - right. eexists; eauto.
+    Qed.
+
+    Theorem derived_closure_set : forall T b e r,
+        derived T
+        -> re_equiv r (derivative b e)
+        -> derived (set_Table T e b r).
+    Proof.
+      intros.
+      (* 1. T' is derived before the set. 
+     2. We know (derivative b e) and r are similar.
+     3. The only entry in T' that changes is the (e, b) entry
+     ---
+     4. T' is still derived after the set.
+       *)
+      unfold derived. intros.
+      (* If e = e0 and a = b, r = r0. Otherwise the entry was there before the set. *)
+      (** may need a hypothesis about getting something that wasn't set **)
+      destruct (regex_eq e e0) eqn:E; destruct (Sigma_dec a b).
+      - apply regex_eq_correct in E. subst.
+        rewrite correct_Table in H1. injection H1; intros; subst.
+        auto.
+      - rewrite moot_setTable in H1; auto.
+      - rewrite moot_setTable in H1; auto.
+        assert(regex_eq e e0 <> true).
+        { intros C. rewrite C in *. discriminate. }
+        right. intros C. destruct H2. apply regex_eq_correct. auto.
+      - rewrite moot_setTable in H1; auto.
+    Qed.
+
+    Theorem derived_closure_add : forall T T' e,
+        derived T
+        -> T' = add_state T e
+        -> derived T'.
+    Proof.
+      unfold derived in *. intros.
+      rewrite H0 in H1. rewrite <- moot_add_state with (r:=e) in H1.
+      apply H in H1. auto.
+    Qed.
+    
+    Lemma derived_closure_ds' : forall bs T T' e n xs,
+        (forall (cs : list Sigma) (e : regex) (T T' : Table),
+            derived T -> T' = fill_Table_all' T e cs n -> derived T')
+        -> derived T
+        ->
+        let
+          fix fill_Table_ds (bs' : list Sigma) : Table :=
+          match bs' with
+          | [] => T
+          | c :: cs =>
+            let T1 := fill_Table_ds cs in
+            let d := canon (derivative c e) in
+            match get_eq T d with
+            | Some e' => set_Table T1 e c e'
+            | None =>
+              let T2 := add_state T1 d in
+              let T3 := set_Table T2 e c d in fill_Table_all' T3 d xs n
+            end
+          end in
+        T' = fill_Table_ds bs
+        -> derived T'.
+    Proof.
+      intros.
+      generalize dependent T.
+      generalize dependent T'.
+      generalize dependent e.
+      generalize dependent xs.
+      induction bs as [|b bs]; intros.
+      - subst; auto.
+      - simpl in H1. repeat dm.
+        + assert(derived (fill_Table_ds bs)).
+          {
+            apply IHbs with (T:=T) (e:=e) (xs:=xs); auto.
+          }
+          apply get_eq_correct in E. destruct E.
+          rewrite H1.
+          apply derived_closure_set; auto.
+          rewrite <- regex_eq_correct in H4. rewrite <- H4.
+          apply canon_equiv.
+        + assert(derived (fill_Table_ds bs)).
+          {
+            apply IHbs with (T:=T) (e:=e) (xs:=xs); auto.
+          }
+          assert(derived (add_state (fill_Table_ds bs) (canon (derivative b e)))).
+          {
+            eapply derived_closure_add; eauto.
+          }
+          clear H2.
+          assert(derived (set_Table
+                            (add_state (fill_Table_ds bs) (canon (derivative b e)))
+                            e b (canon (derivative b e)))).
+          {
+            eapply derived_closure_set; eauto.
+            apply canon_equiv.
+          }
+          eapply H; eauto.
+    Qed.
+    
+    Lemma derived_closure_ds : forall bs T e n xs,
+        (forall (cs : list Sigma) (e : regex) (T T' : Table),
+            derived T -> T' = fill_Table_all' T e cs n -> derived T')
+        -> derived T
+        ->
+        let
+          fix fill_Table_ds (bs' : list Sigma) : Table :=
+          match bs' with
+          | [] => T
+          | c :: cs =>
+            let T1 := fill_Table_ds cs in
+            let d := canon (derivative c e) in
+            match get_eq T d with
+            | Some e' => set_Table T1 e c e'
+            | None =>
+              let T2 := add_state T1 d in
+              let T3 := set_Table T2 e c d in fill_Table_all' T3 d xs n
+            end
+          end in
+        derived (fill_Table_ds bs).
+    Proof.
+      intros. apply derived_closure_ds' with (bs:=bs) (T:=T) (e:=e) (n:=n) (xs:=xs); auto.
+    Qed.
+    
+    
+    Theorem derived_closure_all' : forall n bs e T T',
+        derived T
+        -> T' = fill_Table_all' T e bs n
+        -> derived T'.
+    Proof.
+      induction n; intros; try(simpl in H0; subst; auto; reflexivity).
+      destruct bs as [|b bs].
+      - simpl in H0. subst. auto.
+      - rewrite unfold_filler' in H0. apply unfold_filler_ds in H0. destruct H0.
+        + destruct H0 as (e' & T0 & H0 & H1 & H2).
+          assert(derived T0).
+          {
+            apply derived_closure_ds with (bs:=bs) (xs:= (b :: bs)) (e:=e) (n:=n) in H.
+            subst. auto. apply IHn.
+          }
+          clear H1.
+          subst. eapply derived_closure_set; eauto.
+          apply get_eq_correct in H0. destruct H0.
+          apply regex_eq_correct in H1. rewrite <- H1.
+          apply canon_equiv.
+        + destruct H0 as (T0 & H0 & H1 & H2).
+          assert(derived T0).
+          {
+            apply derived_closure_ds with (bs:=bs) (xs:= (b :: bs)) (e:=e) (n:=n) in H.
+            subst. auto. apply IHn.
+          }
+          clear H1.
+          assert(derived (add_state T0 (canon (derivative b e)))).
+          {
+            eapply derived_closure_add; eauto.
+          }
+          assert(derived (set_Table (add_state T0 (canon (derivative b e)))
+                                    e b (canon (derivative b e)))).
+          {
+            eapply derived_closure_set; eauto.
+            apply canon_equiv.
+          }
+          eapply IHn; eauto.
+    Qed.
+
+    Theorem derived_closure_all : forall n bs e T T',
+        derived T
+        -> T' = fill_Table_all T e bs n
+        -> derived T'.
+    Proof.
+      intros. unfold fill_Table_all in *. eapply derived_closure_all'; eauto.
+    Qed.
+
+    Theorem derived_get_some : forall T e a e',
+        derived T
+        -> get_Table T e a = Some e'
+        -> re_equiv e' (derivative a e).
+    Proof.
+      intros. unfold derived in *. apply H in H0. auto.
+    Qed.
+
+  End Correct.
+
+End DefsFn.
+
+Module Type DefsT (R : regex.T) (TabTy : TABLE R).
+  Include DefsFn R TabTy.
+End DefsT.
+
+Module Type T.
+  Declare Module R : regex.T.
+  Declare Module TabTy : TABLE R.
+  Declare Module Defs : DefsT R TabTy.
+  Export R.
+  Export R.Ty.
+  Export R.Defs.
+  Export TabTy.
+  Export Defs.
+End T.
