Verbatim/DFA/concrete.v
@@ -1,0 +1,185 @@
+Require Import List.
+Import ListNotations.
+
+From Verbatim Require Import ltac.
+From Verbatim Require Import regex.
+From Verbatim Require Import Table.
+
+Module naiveTable (R : regex.T) <: TABLE R.
+
+  Import R.
+  Import R.Ty.
+
+  Definition SigmaMap : Type := list (Sigma * regex).
+
+
+  Fixpoint setSigmaMap (M : SigmaMap) (a : Sigma) (e : regex) : SigmaMap :=
+    match M with
+    | [] => [(a,e)]
+    | (a', e') :: t =>
+      if (Sigma_dec a a')
+      then (a, e) :: t
+      else (a',e') :: (setSigmaMap t a e)
+    end.
+
+  Fixpoint getSigmaMap (M : SigmaMap) (a : Sigma) : option regex :=
+    match M with
+    | [] => None
+    | (a', e') :: t =>
+      if (Sigma_dec a a')
+      then Some e'
+      else getSigmaMap t a
+    end.                                
+
+  Lemma SMget_of_set : forall M e a,
+      getSigmaMap (setSigmaMap M a e) a = Some (e).
+  Proof.
+    induction M; intros; auto.
+    - simpl. dm. contradiction.
+    - simpl. repeat dm.
+      + simpl. dm. contradiction.
+      + simpl. destruct (Sigma_dec a0 s) eqn:E1.
+        * contradiction.
+        * auto.
+  Qed.
+
+  Lemma SMmoot_set : forall M a b r,
+      a <> b
+      -> getSigmaMap (setSigmaMap M b r) a = getSigmaMap M a.
+  Proof.
+    induction M; intros.
+    - simpl. dm. contradiction.
+    - simpl. repeat dm; subst; try(contradiction).
+      + simpl. dm. contradiction.
+      + simpl. dm. contradiction.
+      + simpl. dm. contradiction.
+  Qed.
+
+
+
+  Definition RegexMap : Type := list (regex * SigmaMap).
+
+  Fixpoint setRegexMap (M : RegexMap) (e : regex) (SM : SigmaMap) :=
+    match M with
+    | [] => [(e,SM)]
+    | (e', SM') :: t =>
+      if (regex_dec e e')
+      then (e, SM) :: t
+      else (e', SM') :: (setRegexMap t e SM)
+    end.
+
+  Fixpoint getRegexMap (M : RegexMap) (e : regex) : option SigmaMap :=
+    match M with
+    | [] => None
+    | (e', SM') :: t =>
+      if (regex_dec e e')
+      then Some SM'
+      else getRegexMap t e
+    end.    
+
+  Lemma RMget_of_set : forall RM e SM,
+      getRegexMap (setRegexMap RM e SM) e = Some (SM).
+  Proof.
+    induction RM; intros.
+    - simpl. dm. contradiction.
+    - simpl. repeat (dm; simpl); try(contradiction).
+  Qed.
+
+  Lemma RMset_moot : forall RM e e' SM,
+      e' <> e
+      ->  getRegexMap (setRegexMap RM e SM) e' = getRegexMap RM e'.
+  Proof.
+    induction RM; intros.
+    - simpl. dm. contradiction.
+    - simpl. repeat (dm; simpl); try(contradiction).
+      clear E1. rewrite e1 in n. rewrite e0 in n. contradiction.
+  Qed.
+
+
+  Definition Table : Type := (RegexMap * list regex).
+  Definition emptyTable : Table := ([],[]).
+
+  Fixpoint set_Table (T : Table) (e : regex) (a : Sigma) (e' : regex) : Table :=
+    match getRegexMap (fst T) e with
+    | None => (setRegexMap (fst T) e (setSigmaMap [] a e'), snd T)
+    | Some SM => (setRegexMap (fst T) e (setSigmaMap SM a e'), snd T)
+    end.
+
+  Fixpoint get_Table (T : Table) (e : regex) (a : Sigma) : option regex :=
+    match getRegexMap (fst T) e with
+    | None => None
+    | Some SM => getSigmaMap SM a
+    end.
+
+
+  Lemma foo : forall T e a r,
+      set_Table T e a r
+      = match getRegexMap (fst T) e with
+        | None => (setRegexMap (fst T) e (setSigmaMap [] a r), snd T)
+        | Some SM => (setRegexMap (fst T) e (setSigmaMap SM a r), snd T)
+        end.
+  Proof.
+    intros. destruct T; auto.
+  Qed.
+
+  Lemma bar : forall T e a,
+      get_Table T e a
+      = match getRegexMap (fst T) e with
+        | None => None
+        | Some SM => getSigmaMap SM a
+        end.
+  Proof.
+    intros. destruct T; auto.
+  Qed.
+
+  Lemma correct_Table : forall T e a r, get_Table (set_Table T e a r) e a = Some (r).
+  Proof.
+    intros. rewrite bar. rewrite foo. destruct (getRegexMap (fst T) e) eqn:E.
+    - dm.
+      + simpl in E0. rewrite RMget_of_set in E0. injection E0; intros; subst.
+        rewrite SMget_of_set. auto.
+      + simpl in E0. rewrite RMget_of_set in *. discriminate.
+    - dm.
+      + simpl in E0. rewrite RMget_of_set in *.
+        assert(s = setSigmaMap [] a r).
+        { injection E0; intros; subst; auto. }
+        rewrite H.
+        rewrite SMget_of_set. auto.
+      + simpl in E0. rewrite RMget_of_set in *. discriminate.
+  Qed.
+
+  Lemma moot_setTable : forall T e0 e a b r,
+      a <> b
+      \/ e <> e0
+      -> get_Table (set_Table T e b r) e0 a = get_Table T e0 a.
+  Proof.
+    intros. rewrite bar. rewrite foo. destruct (getRegexMap (fst T) e) eqn:E.
+  Admitted.
+
+  Lemma correct_emptyTable : forall e a, get_Table emptyTable e a = None.
+  Proof.
+    auto.
+  Qed.
+
+  Definition add_state (T : Table) (e : regex) : Table :=
+    match T with
+    | (T', sts) => (T', e :: sts)
+    end.
+
+  Definition get_states (T : Table) := snd T.
+
+  Lemma empty_states : get_states emptyTable = [].
+  Proof. auto. Qed.
+
+  Lemma correct_states : forall T r, In r (get_states (add_state T r)).
+  Proof.
+    intros. destruct T. simpl. auto.
+  Qed.
+
+  Lemma moot_add_state : forall T e a r,
+      get_Table T e a = get_Table (add_state T r) e a.
+  Proof.
+    intros. destruct T. auto.
+  Qed.
+
+End naiveTable.
