Verbatim/matcher.v
@@ -18,97 +18,9 @@ End ImplFn.
 Module LemmasFn (Import R : regex.T).
   
   Include ImplFn R.
+  Import R.Ty.
   
   { (**)
-    
-    Theorem nullable_bridge : forall(r : regex),
-      true = nullable r <-> exp_match [] r.
-    Proof.
-      intros r. split; intros H.
-      - induction r; try(simpl in H; discriminate).
-        + apply MEmpty.
-        + simpl in H. destruct (nullable r1); destruct (nullable r2); try(simpl in H; discriminate).
-          rewrite <- nil_left with (s := []). apply MApp.
-          * apply IHr1. reflexivity.
-          * apply IHr2. reflexivity.
-        + simpl in H.  destruct (nullable r1); destruct (nullable r2).
-          * apply MUnionL. apply IHr1. reflexivity.
-          * apply MUnionL. apply IHr1. reflexivity.
-          * apply MUnionR. apply IHr2. reflexivity.
-          * simpl in H. discriminate.
-        + apply MStar0.
-      - induction r.
-        + inversion H.
-        + simpl. reflexivity.
-        + inversion H.
-        + simpl. inversion H. apply empty_app in H1. destruct H1.
-          rewrite H1 in H3. rewrite H5 in H4.
-          apply IHr1 in H3. apply IHr2 in H4.
-          rewrite <- H3. rewrite <- H4. simpl. reflexivity.
-        + simpl. inversion H.
-          * apply IHr1 in H2. rewrite <- H2. destruct (nullable r2); simpl; reflexivity.
-          * apply IHr2 in H1. rewrite <- H1. destruct (nullable r1); simpl; reflexivity.
-        + simpl. reflexivity.
-    Qed.
-
-    Theorem nullable_bridge' : forall(r : regex),
-        nullable r = true <-> exp_match [] r.
-    Proof.
-      split; intros.
-      - symmetry in H. apply nullable_bridge; auto.
-      - symmetry. apply nullable_bridge; auto.
-    Qed.
-
-    (* star_concat upto concat_star necessary for hard star case of der_match *)
-    Lemma star_concat :
-      forall s r',
-        exp_match s (Star r')
-        -> (exists xss : list (list Sigma),
-               s = concat xss
-               /\ (forall xs,
-                      In xs xss
-                      -> exp_match xs r')).
-    Proof.
-      intros s r' hm.
-      remember (Star r') as r. generalize dependent r'.
-      induction hm; intros r' heq; inv heq.
-      - exists []; split; auto.
-        intros xs hi; inv hi.
-      - destruct (IHhm2 r') as (xss' & heq & hall); subst; auto.
-        exists (s1 :: xss'); split; auto.
-        intros xs hi.
-        destruct hi as [hh| ht]; subst; auto.
-    Qed.
-
-    Lemma star_concat_no_empt : forall(s : String) (r' : regex),
-        s <> []
-        -> exp_match s (Star r')
-        -> (exists xss : list (list Sigma),
-               s = concat xss
-               /\ (forall xs,
-                      In xs xss
-                      -> exp_match xs r' /\ xs <> [])).
-    Proof.
-      intros s r' Hempty Hstar. apply star_concat in Hstar.
-      destruct Hstar as (yss & heq & hall).
-      exists(rm_empty yss). split.
-      - rewrite rm_empty_mute. apply heq.
-      - intros xs H. split.
-        + apply hall.  apply filtered_subset in H. apply H.
-        + apply rm_empty_no_empty in H. apply H.
-    Qed.
-
-    Lemma concat_star : forall(xss : list String) (r : regex),
-        (forall xs : list Sigma, In xs xss -> exp_match xs r) -> exp_match (concat xss) (Star r).
-    Proof.
-      intros xss r H. induction xss.
-      - simpl. apply MStar0.
-      - replace (concat (a :: xss)) with (a ++ (concat xss)).
-        + apply MStarApp.
-          * apply H. simpl. left. reflexivity.
-          * apply IHxss. intros xs H1. apply H. simpl. right. apply H1.
-        + simpl. reflexivity.
-    Qed.
 
     Theorem der_matchb : forall(a : Sigma) (s : String) (r : regex),
         true = exp_matchb (a::s) r <-> true = exp_matchb s (derivative a r).
@@ -123,6 +35,7 @@ End LemmasFn.
 Module CorrectFn (Import R : regex.T).
 
   Include LemmasFn R.
+  Import R.Ty.
 
   { (**)
 
@@ -134,105 +47,6 @@ Module CorrectFn (Import R : regex.T).
       - symmetry. rewrite false_not_true in *.
         intros C. destruct E.
         symmetry in C. rewrite <- der_matchb in C. auto.
-    Qed.
-    
-    Theorem der_match : forall(a : Sigma) (s : String) (r : regex),
-        exp_match (a::s) r <-> exp_match s (derivative a r).
-    Proof.
-      intros a s r.
-      split.
-      {
-        generalize dependent s. induction r; intros s H.
-        - inv H.
-        - inv H.
-        - destruct s.
-          + simpl. destruct (R.Ty.Sigma_dec t a).
-            * apply MEmpty.
-            * inv H. contradiction.
-          + inv H.
-        - simpl. destruct(nullable r1) eqn:E.
-          + inv H. destruct s1.
-            * apply MUnionR. apply IHr2. rewrite <- H1. simpl. apply H4.
-            * apply MUnionL. simpl in H1. injection H1. intros Happ Hchar.
-              rewrite <- Happ. rewrite Hchar in H3. apply IHr1 in H3.
-              apply MApp.
-              -- apply H3.
-              -- apply H4.
-          + inv H. destruct s1.
-            * apply nullable_bridge in H3. rewrite E in H3. discriminate.
-            * simpl in H1. injection H1. intros Happ Hchar.
-              rewrite <- Happ. rewrite Hchar in H3. apply IHr1 in H3.
-              apply MApp.
-              -- apply H3.
-              -- apply H4.
-        - simpl. inv H.
-          + apply IHr1 in H2. apply MUnionL. apply H2.
-          + apply IHr2 in H1. apply MUnionR. apply H1.
-        (* hard_star: This case was the hard one *)
-        - apply star_concat_no_empt in H. destruct H as (xss & heq & hall).
-          + assert (H : exists(s1 : String) (yss : list String),
-                       ((a :: s1) :: yss) = xss).
-            {
-              destruct xss.
-              - simpl in heq. discriminate.
-              - simpl in heq. destruct l eqn:E.
-                + apply hall in E.
-                  * contradiction.
-                  * rewrite E. simpl. left. reflexivity.
-                + exists(l0). exists(xss). simpl in heq.
-                  injection heq. intros I1 I2. rewrite I2. reflexivity.
-            }
-            destruct H as [s1]. destruct H as [yss].
-            rewrite <- H in hall.
-            assert (A : In (a :: s1) ((a :: s1) :: yss)).
-            { simpl. left. reflexivity. }
-            simpl. replace s with (s1 ++ (concat yss)).
-            * apply MApp.
-              -- apply IHr. apply hall in A. destruct A. apply H0.
-              -- rewrite H in hall.
-                 assert (A1 : forall xs : list Sigma, In xs xss -> exp_match xs r).
-                 { intros xs. intros HA1. apply hall in HA1. destruct HA1. apply H0. }
-                 apply concat_star. intros xs H1. apply A1.
-                 rewrite <- H. simpl. right. apply H1.
-            * assert (A1 : concat ((a :: s1) :: yss) = concat xss).
-              { rewrite H. reflexivity. }
-              assert (A2 : concat ((a :: s1) :: yss) = a :: (s1 ++ (concat yss))).
-              { simpl. reflexivity. }
-              rewrite <- A1 in heq. rewrite A2 in heq. injection heq.
-              intros I. symmetry. apply I.
-          + unfold not. intros C. discriminate.
-      }
-      {
-        generalize dependent s. induction r; intros s H.
-        - inv H.
-        - inv H.
-        - simpl in H. destruct (R.Ty.Sigma_dec t a); inv H. apply MChar.
-        - simpl in H. destruct (nullable r1) eqn:E.
-          + inv H.
-            * inv H2. replace (a :: s1 ++ s2) with ((a :: s1) ++ s2).
-              apply MApp.
-              -- apply IHr1. apply H3.
-              -- apply H4.
-              -- reflexivity.
-            * symmetry in E. apply nullable_bridge in E. rewrite <- nil_left with (s := (a :: s)).
-              apply MApp.
-              -- apply E.
-              -- apply IHr2. apply H1.
-          + inv H.
-            * replace (a :: s1 ++ s2) with ((a :: s1) ++ s2).
-              apply MApp.
-              -- apply IHr1. apply H3.
-              -- apply H4.
-              -- reflexivity.
-        - inv H.
-          + apply MUnionL. apply IHr1. apply H2.
-          + apply MUnionR. apply IHr2. apply H1.
-        - simpl in H. inv H. replace (a :: s1 ++ s2) with ((a :: s1) ++ s2).
-          + apply MStarApp.
-            * apply IHr. apply H3.
-            * apply H4.
-          + reflexivity.
-      }
     Qed.
 
     Theorem match_iff_matchb : forall(s : String) (r : regex),
