Evaluation/Example/README.md
@@ -1,0 +1,29 @@
+# Performance Evaluation
+
+## Compilation
+First compile Verbatim according to "../README.md". This will automatically extract the relevant code from Coq to OCaml and place it in the proper directory.
+
+Then compile the evaluation executable:
+~~~
+ocamlopt -O3 -w -20 -w -26 -o instancedriver instance.mli instance.ml instancedriver.ml
+~~~
+We compiled using the 4.11.0+flambda version of OCaml.
+
+## I/O
+~~~
+mkdir data results
+~~~
+Place your input json data into the data folder. The results will be placed in the results folder.
+
+## Execution
+To execute the evaluation driver, run
+~~~
+./instancedriver
+~~~
+
+## Visualization
+Once the driver has finished executing, the results can be visualized with
+~~~
+python3 plot.py
+~~~
+This requires the python3 libraries matplotlib and numpy.
